src/theory/NRGTNFLemmas.v
@@ -16,7 +16,6 @@ Require Import SchemaWellFormedness.
 Require Import Schema.
 Require Import SchemaAux.
 
-Require Import QueryConformance.
 
 Require Import SeqExtra.
 
@@ -34,8 +33,50 @@ Section Theory.
 
   Section Ground.
     Variable (s : @wfGraphQLSchema Vals).
+
+    (**
+       Elimination lemma for [are_grounded_fields].
+     *)
+    Lemma are_grounded_fields_E φ :
+      are_grounded_fields s φ = all (fun q => q.(is_field)) φ && all (is_grounded s) φ.
+    Proof.
+      elim: φ => //= q φ ->.
+        by rewrite andbACA -[RHS]andbA.
+    Qed.
+
+    (**
+       This lemma states that if some queries [are_grounded_fields] then 
+       they [are_grounded].
+     *)
+    Lemma are_grounded_fields_grounded φ :
+      are_grounded_fields s φ ->
+      are_grounded s φ.
+    Proof.
+        by case: φ => //= q φ; case_query q.
+    Qed.
+
+    (**
+       Elimination lemma for [are_grounded_fields].
+     *)
+    Lemma are_grounded_inlines_E qs : are_grounded_inlines s qs = all (fun q => q.(is_inline_fragment)) qs && all (is_grounded s) qs.
+    Proof.
+      elim: qs => //= q qs ->.
+        by rewrite andbACA -[RHS]andbA.
+    Qed.
+
+    (**
+       This lemma states that if some queries [are_grounded_inlines] then 
+       they [are_grounded].
+     *)
+    Lemma are_grounded_inlines_grounded φ :
+      are_grounded_inlines s φ ->
+      are_grounded s φ.
+    Proof.
+        by case: φ => //= q φ; case_query q.
+    Qed.
+
+      
     
-   
     (**
        This lemma states that the predicate [are_grounded2] distributes over list concatenation.
      *)
@@ -94,26 +135,7 @@ Section Theory.
     Qed.
 
 
-    (**
-       Elimination lemma for [are_grounded_fields].
-     *)
-    Lemma are_grounded_fields_E qs :
-      are_grounded_fields s qs = all (fun q => q.(is_field)) qs && all (is_grounded s) qs.
-    Proof.
-      elim: qs => //= q qs ->.
-        by rewrite andbACA -[RHS]andbA.
-    Qed.
-
-    (**
-       This lemma states that if queries [are_grounded_fields] then they 
-       [are_grounded].
-     *)
-    Lemma are_grounded_fields_grounded φ :
-      are_grounded_fields s φ -> are_grounded s φ.
-    Proof.
-        by elim: φ => //= q φ IH /and3P [-> Hg Hgs]; apply_andP.
-    Qed.
-
+   
 
     Section Filter.
 
@@ -171,11 +193,31 @@ Section Theory.
 
   Section NonRedundant.
 
+    
+    Implicit Type φ : seq (@Query Vals).
 
+    
     Section Filter.
 
-      
-      
+      Transparent qresponse_name.
+           
+
+      (**
+         This lemma states that filtering according to a response name preserves non-redundancy
+         of the queries.
+       *)
+      Lemma filter_preserves_non_redundancy rname φ :
+        are_non_redundant φ ->
+        are_non_redundant (filter_queries_with_label rname φ).
+      Proof.
+        funelim (filter_queries_with_label rname φ) => //=; simp are_non_redundant; bcase; do ? by apply: H.
+        all: do [apply_and3P].
+        all: do ? by apply/eqP; apply: filter_preserves_find_frags_nil; apply/eqP.
+        all: do ? by apply: H.
+        all: do ? by apply: H0.
+        all: do [by apply/eqP; apply: filter_preserves_find_fields_nil; apply/eqP].
+      Qed.
+        
     End Filter.
 
   End NonRedundant.
@@ -183,6 +225,29 @@ Section Theory.
   
 End Theory.
 
+
+ Ltac grounding :=
+    repeat match goal with
+           (* | [|- context [are_grounded (_ ++ _)] ] => rewrite are_grounded_cat *)
+           | [|- is_true (are_grounded _ (filter_queries_with_label _ _))] =>
+             apply: filter_preserves_grounding
+                      
+           | [H : ?P |- ?P] => exact: H
+           | [H : is_true (are_grounded_fields _ ?φ) |- is_true (are_grounded _ ?φ)] => by apply: are_grounded_fields_grounded
+           | [H : is_true (are_grounded_inlines _ ?φ) |- is_true (are_grounded _ ?φ)] => by apply: are_grounded_inlines_grounded
+          
+           | [|- context [are_grounded _ (_ :: _)] ] => rewrite are_grounded_equation_2 /=
+           (* | [|- context [is_grounded _ _] ] => simp is_grounded *)
+           end.
+
+  Ltac non_red :=
+    repeat match goal with
+           | [|- is_true (are_non_redundant (filter_queries_with_label _ _))] =>
+               by apply: filter_preserves_non_redundancy
+           | [|- context [are_non_redundant (_ :: _)] ] => simp are_non_redundant
+           | [|- is_true (are_non_redundant (_ :: _)) -> _] => simp are_non_redundant
+           | [|- is_true (are_non_redundant _)] => simp are_non_redundant
+           end.
 
 
 
