src/theory/QuerySemanticsLemmas.v
@@ -59,8 +59,75 @@ Section Theory.
         let v := fresh "v" in
         let vs := fresh "vs" in
         case Hv : (field_seq_value u.(nfields) _) => [ [v | vs] |] /=
+
+      | [H : (return_type ?f) = _ |- context [ return_type ?f ] ] => rewrite H /=
+
+      | [|- context[ execute_selection_set_unfold_clause_4_clause_1 _ _ _ _ (return_type ?fld)] ] =>
+        let Hrty := fresh "Hrty" in
+        let rty := fresh "rty" in
+        case Hrty : fld.(return_type) => [rty | rty] /=
+
+      | [|- context[ execute_selection_set_unfold_clause_4_clause_1_clause_2 _ _ _ _ _ _ (ohead _)] ] =>
+        let Hv := fresh "Hv" in
+        case Hv : ohead => [v|] //=
+                               
+      | [|- context[ execute_selection_set_unfold_clause_5_clause_1 _ _ _ _ (return_type ?fld)] ] =>
+        let Hrty := fresh "Hrty" in
+        let rty := fresh "rty" in
+        case Hrty : fld.(return_type) => [rty | rty] /=
+
+      | [|- context[ execute_selection_set_unfold_clause_5_clause_1_clause_2 _ _ _ _ _ _ (ohead _)] ] =>
+        let Hv := fresh "Hv" in
+        case Hv : ohead => [v|] //=
+                               
       | [ H : does_fragment_type_apply _ _ _ = _ |- context [ does_fragment_type_apply _ _ _] ] => rewrite H /=
+
+      | [|- context [execute_selection_set_unfold_clause_6 _ _ _ _ _ (does_fragment_type_apply _ _ _)] ] =>
+        let Hfapplies := fresh "Hfapplies" in
+        case Hfapplies : does_fragment_type_apply => //=
+   
       | [ |- context [ _, _ ⊢ ⟦ _ ⟧ˢ in _ ] ] => simp execute_selection_set
+      end.
+
+  Ltac exec2 :=
+    repeat
+      match goal with
+      | [ H : lookup_field_in_type _ _ _ = _ |- context [ lookup_field_in_type _ _ _] ] => rewrite H /=
+      | [ H : (field_seq_value (nfields _) _) = _ |- context [ field_seq_value (nfields _) _] ] => rewrite H /=
+
+      | [|- context [ lookup_field_in_type _ _ _] ] => lookup
+      | [|- context [ field_seq_value ?u.(nfields) ] ] =>
+        let Hv := fresh "Hv" in
+        let v := fresh "v" in
+        let vs := fresh "vs" in
+        case Hv : (field_seq_value u.(nfields) _) => [ [v | vs] |] /=
+
+      | [H : (return_type ?f) = _ |- context [ return_type ?f ] ] => rewrite H /=
+
+      | [H : (return_type ?f) = _ |- context [ return_type ?f ] ] => rewrite H /=
+
+      | [|- context[ execute_selection_set2_unfold_clause_4_clause_1 _ _ _ _ (return_type ?fld)] ] =>
+        let Hrty := fresh "Hrty" in
+        let rty := fresh "rty" in
+        case Hrty : fld.(return_type) => [rty | rty] /=
+
+      | [|- context[ execute_selection_set2_unfold_clause_4_clause_1_clause_2 _ _ _ _ _ _ (ohead _)] ] =>
+        let Hv := fresh "Hv" in
+        case Hv : ohead => [v|] //=
+     
+      | [|- context[ execute_selection_set2_unfold_clause_5_clause_1 _ _ _ _ (return_type ?fld)] ] =>
+        let Hrty := fresh "Hrty" in
+        let rty := fresh "rty" in
+        case Hrty : fld.(return_type) => [rty | rty] /=
+
+      | [|- context[ execute_selection_set2_unfold_clause_5_clause_1_clause_2 _ _ _ _ _ _ (ohead _)] ] =>
+        let Hv := fresh "Hv" in
+        case Hv : ohead => [v|] //=
+     
+      | [H : (ohead (neighbours_with_field _ _ _)) = _ |- context [ ohead (neighbours_with_field _ _ _)] ] =>
+        rewrite H /=
+      | [ H : does_fragment_type_apply _ _ _ = _ |- context [ does_fragment_type_apply _ _ _] ] => rewrite H /=
+      | [ |- context [ _, _ ⊢ ≪ _ ≫ in _ ] ] => simp execute_selection_set2
       end.
 
 
@@ -76,7 +143,7 @@ Section Theory.
   Proof.
     elim: ptys => //= t ptys IH /andP [Hnin Huniq] /andP [Hobj Hinobj] Hunin.
     have /negbTE Hneq : u.(ntype) != t by move/memPn: Hunin => /(_ t (mem_head t ptys)); rewrite eq_sym.
-    exec; rewrite /does_fragment_type_apply Hobj Hneq /=.
+    simp execute_selection_set; rewrite /does_fragment_type_apply Hobj Hneq /=.
     apply: IH => //=.
     move: Hunin; rewrite /negb; case: ifP => //=.
       by case: ifP => //= Hin <- _; apply: mem_tail.
@@ -110,31 +177,18 @@ Section Theory.
       
       
       case_query q; simp query_size => Hleq Hobj Hunin; exec;
-                                        rewrite ?filter_queries_with_label_cat ?filter_map_inline_func ?Hinlineswap.
-      all: do ? by congr cons; apply: IH; leq_queries_size.
+                                        rewrite ?filter_queries_with_label_cat ?filter_map_inline_func ?Hinlineswap ?IH //; leq_queries_size.
+      (* all: do ? by congr cons; apply: IH; leq_queries_size. *)
 
-    - case fld.(return_type) => //= rty.
-      * case ohead => [v|] //=; rewrite filter_queries_with_label_cat filter_map_inline_func Hinlineswap IH //; leq_queries_size.
-        congr cons; congr pair; congr Response.Object.
-          by rewrite find_queries_with_label_cat find_map_inline_nil_func // cats0.
+    - by congr cons; congr pair; congr Response.Object; rewrite find_queries_with_label_cat find_map_inline_nil_func // cats0.
+        
+    - by congr cons; rewrite find_queries_with_label_cat find_map_inline_nil_func // cats0.
 
-      * rewrite filter_queries_with_label_cat filter_map_inline_func Hinlineswap IH //; leq_queries_size.
-        rewrite find_queries_with_label_cat find_map_inline_nil_func // cats0.
-          by congr cons; congr pair; congr Array.
+    - by congr cons; congr pair; congr Response.Object; rewrite find_queries_with_label_cat find_map_inline_nil_func // cats0.
 
-    - by apply: IH; leq_queries_size.
+    - by congr cons; rewrite find_queries_with_label_cat find_map_inline_nil_func // cats0.
 
-    - case fld.(return_type) => //= rty.
-      * case ohead => [v|] //=; rewrite filter_queries_with_label_cat filter_map_inline_func Hinlineswap IH //; leq_queries_size.
-        congr cons; congr pair; congr Response.Object.
-          by rewrite find_queries_with_label_cat find_map_inline_nil_func // cats0.
-      * rewrite filter_queries_with_label_cat filter_map_inline_func Hinlineswap IH //; leq_queries_size.
-        rewrite find_queries_with_label_cat find_map_inline_nil_func // cats0.
-          by congr cons; congr pair; congr Array.
-
-    - by apply: IH; leq_queries_size.
-
-    - by case: does_fragment_type_apply => //=; rewrite ?catA; apply: IH => //; leq_queries_size.
+    - by rewrite catA; apply: IH => //; leq_queries_size.
   Qed.
   
   Lemma exec_cat_frags ptys u φ1 φ2 :
@@ -166,7 +220,7 @@ Section Theory.
     move=> Hswap.
     elim: ptys => //= t ptys IH /andP [Hnin Huniq] /andP [Hobj Hinobj].
     rewrite inE => /orP [/eqP Heq | Hin].
-    - rewrite -Heq in Hnin *; exec.
+    - rewrite -Heq in Hnin *; simp execute_selection_set.
       have -> /= : does_fragment_type_apply s u.(ntype) u.(ntype).
         by apply: object_applies_to_itself; rewrite Heq; apply: Hobj.
           by rewrite cats0; apply: exec_cat_frags_func.
@@ -199,50 +253,42 @@ Section Theory.
           s, g ⊢ ⟦ normalize s u.(ntype) φ ⟧ˢ in u =  s, g ⊢ ⟦ φ ⟧ˢ in u.
   Proof.    
     funelim (normalize s u.(ntype) φ) => //=; do ? by exec.
-    all: do ? [by intros; exec; rewrite filter_normalize_swap filter_filter_absorb // H].
-    - move=> Huin; exec.
-      case Hrty : f.(return_type) => [rty| rty] /=.
-      * case Hv : ohead => [v|] //=;
-                               rewrite filter_normalize_swap filter_filter_absorb // H0 // -filter_normalize_swap find_filter_nil.
-        simp merge_selection_sets => /=; rewrite cats0.
-        rewrite Hrty /= in H.
-        congr cons; congr pair; congr Response.Object.
-        have Hvin : v \in g.(nodes).
+    all: do ? [by intros; exec; rewrite filter_normalize_swap filter_filter_absorb // H]; exec => Huin.
+
+    all: do ? [rewrite filter_normalize_swap filter_filter_absorb // H0 // -?filter_normalize_swap find_queries_filter_nil].
+    - simp merge_selection_sets => /=; rewrite cats0.
+      rewrite Hrty /= in H.
+      congr cons; congr pair; congr Response.Object.
+      have Hvin : v \in g.(nodes).
         apply: ohead_in_nodes; last by apply: Hv.
         apply/allP.
           by apply: neighbours_are_in_nodes.
-          have Hvtype : v.(ntype) = rty.
-          rewrite Hrty /= in Heq.
-          apply: (in_object_possible_types Heq).
-          have Hlook : lookup_field_in_type s u.(ntype) (Field name1 arguments1) = Some f by [].
-          move/ohead_in: Hv => Hin.
-          move: (@neighbours_are_subtype_of_field Vals s g u (Field name1 arguments1) f Hlook v Hin).
-            by rewrite Hrty.
-              by apply: H => //; rewrite Hvtype.
-              
-              
-      * rewrite filter_normalize_swap filter_filter_absorb // H0 //; congr cons; congr pair; congr Array.
-        apply/eq_in_map => v Hin; congr Response.Object.
-        rewrite -filter_normalize_swap find_filter_nil.
-        simp merge_selection_sets => /=; rewrite cats0.
-        rewrite Hrty /= in H.
-        have Hvin : v \in g.(nodes).
+      have Hvtype : v.(ntype) = rty.
+        rewrite Hrty /= in Heq.
+        apply: (in_object_possible_types Heq).
+        have Hlook : lookup_field_in_type s u.(ntype) (Field name1 arguments1) = Some f by [].
+        move/ohead_in: Hv => Hin.
+        move: (@neighbours_are_subtype_of_field Vals s g u (Field name1 arguments1) f Hlook v Hin).
+          by rewrite Hrty.
+      by apply: H => //; rewrite Hvtype.
+      
+    - congr cons; congr pair; congr Array.
+      apply/eq_in_map => v Hin; congr Response.Object.
+      simp merge_selection_sets => /=; rewrite cats0.
+      rewrite Hrty /= in H.
+      have Hvin : v \in g.(nodes).
         apply: neighbours_are_in_nodes; exact: Hin.
-        have Hvtype : v.(ntype) = rty.
+      have Hvtype : v.(ntype) = rty.
         rewrite Hrty in Heq; apply: (in_object_possible_types Heq).
         have Hlook : lookup_field_in_type s u.(ntype) (Field name1 arguments1) = Some f by [].
         move: (@neighbours_are_subtype_of_field Vals s g u (Field name1 arguments1) f Hlook v Hin).
           by rewrite Hrty /=. (* ?? *)
-            by apply: H => //; rewrite Hvtype.
+      by apply: H => //; rewrite Hvtype.
             
-    - move=> Huin; exec.
-      case Hrty : f.(return_type) => [rty | rty] //=.
-      * case Hv : ohead => [v|] /=; rewrite filter_normalize_swap filter_filter_absorb // H0 //.
-        rewrite -filter_normalize_swap find_filter_nil.
-        simp merge_selection_sets => /=; rewrite cats0.
+    - simp merge_selection_sets => /=; rewrite cats0.
         congr cons; congr pair; congr Response.Object.
         rewrite exec_inlined_func //.
-        exec.
+        simp execute_selection_set.
         have Hvin : v \in g.(nodes).
         apply: ohead_in_nodes; last by apply: Hv.
           by apply/allP; apply: neighbours_are_in_nodes.
@@ -259,11 +305,10 @@ Section Theory.
                   move: (@neighbours_are_subtype_of_field Vals s g u (Field name1 arguments1) f Heq0 v Hin).
                     by rewrite Hrty.
                     
-      * rewrite filter_normalize_swap filter_filter_absorb // H0 //; congr cons; congr pair; congr Array.
+      * congr cons; congr pair; congr Array.
         apply/eq_in_map => v Hin; congr Response.Object.
-        rewrite -filter_normalize_swap find_filter_nil.
         simp merge_selection_sets => /=; rewrite cats0 exec_inlined_func.
-        exec.
+        simp execute_selection_set.
         have Hvin : v \in g.(nodes) by apply: neighbours_are_in_nodes; exact: Hin.
         have Hvobj := (node_in_graph_has_object_type Hvin).
         have -> /= : does_fragment_type_apply s v.(ntype) v.(ntype) by apply: object_applies_to_itself.
@@ -277,82 +322,72 @@ Section Theory.
                   by rewrite Hrty.
                   
 
-    - move=> Huin; exec.
-      case Hrty : f.(return_type) => [rty| rty] /=.
-      * case Hv : ohead => [v|] //=;
-                               rewrite filter_normalize_swap filter_filter_absorb // H0 // -filter_normalize_swap find_filter_nil.
-        simp merge_selection_sets => /=; rewrite cats0.
-        rewrite Hrty /= in H.
-        congr cons; congr pair; congr Response.Object.
-        have Hvin : v \in g.(nodes).
-        apply: ohead_in_nodes; last by apply: Hv.
-        apply/allP.
-          by apply: neighbours_are_in_nodes.
-          have Hvtype : v.(ntype) = rty.
-          rewrite Hrty /= in Heq.
-          apply: (in_object_possible_types Heq).
-          have Hlook : lookup_field_in_type s u.(ntype) (Field name2 arguments2) = Some f by [].
-          move/ohead_in: Hv => Hin.
-          move: (@neighbours_are_subtype_of_field Vals s g u (Field name2 arguments2) f Hlook v Hin).
-            by rewrite Hrty.
-              by apply: H => //; rewrite Hvtype.
+    - simp merge_selection_sets => /=; rewrite cats0.
+      rewrite Hrty /= in H.
+      congr cons; congr pair; congr Response.Object.
+      have Hvin : v \in g.(nodes).
+      apply: ohead_in_nodes; last by apply: Hv.
+      apply/allP.
+        by apply: neighbours_are_in_nodes.
+      have Hvtype : v.(ntype) = rty.
+      rewrite Hrty /= in Heq.
+      apply: (in_object_possible_types Heq).
+      have Hlook : lookup_field_in_type s u.(ntype) (Field name2 arguments2) = Some f by [].
+      move/ohead_in: Hv => Hin.
+      move: (@neighbours_are_subtype_of_field Vals s g u (Field name2 arguments2) f Hlook v Hin).
+        by rewrite Hrty.
+          by apply: H => //; rewrite Hvtype.
               
               
-      * rewrite filter_normalize_swap filter_filter_absorb // H0 //; congr cons; congr pair; congr Array.
-        apply/eq_in_map => v Hin; congr Response.Object.
-        rewrite -filter_normalize_swap find_filter_nil.
-        simp merge_selection_sets => /=; rewrite cats0.
-        rewrite Hrty /= in H.
-        have Hvin : v \in g.(nodes).
-        apply: neighbours_are_in_nodes; exact: Hin.
-        have Hvtype : v.(ntype) = rty.
-        rewrite Hrty in Heq; apply: (in_object_possible_types Heq).
-        have Hlook : lookup_field_in_type s u.(ntype) (Field name2 arguments2) = Some f by [].
-        move: (@neighbours_are_subtype_of_field Vals s g u (Field name2 arguments2) f Hlook v Hin).
-          by rewrite Hrty /=. (* ?? *)
-            by apply: H => //; rewrite Hvtype.
+    - congr cons; congr pair; congr Array.
+      apply/eq_in_map => v Hin; congr Response.Object.
+      simp merge_selection_sets => /=; rewrite cats0.
+      rewrite Hrty /= in H.
+      have Hvin : v \in g.(nodes).
+      apply: neighbours_are_in_nodes; exact: Hin.
+      have Hvtype : v.(ntype) = rty.
+      rewrite Hrty in Heq; apply: (in_object_possible_types Heq).
+      have Hlook : lookup_field_in_type s u.(ntype) (Field name2 arguments2) = Some f by [].
+      move: (@neighbours_are_subtype_of_field Vals s g u (Field name2 arguments2) f Hlook v Hin).
+        by rewrite Hrty /=. (* ?? *)
+          by apply: H => //; rewrite Hvtype.
             
-    - move=> Huin; exec.
-      case Hrty : f.(return_type) => [rty | rty] //=.
-      * case Hv : ohead => [v|] /=; rewrite filter_normalize_swap filter_filter_absorb // H0 //.
-        rewrite -filter_normalize_swap find_filter_nil.
-        simp merge_selection_sets => /=; rewrite cats0.
-        congr cons; congr pair; congr Response.Object.
-        rewrite exec_inlined_func //.
-        exec.
-        have Hvin : v \in g.(nodes).
-        apply: ohead_in_nodes; last by apply: Hv.
-          by apply/allP; apply: neighbours_are_in_nodes.
-          have Hvobj := (node_in_graph_has_object_type Hvin).
-          have -> /= : does_fragment_type_apply s v.(ntype) v.(ntype) by apply: object_applies_to_itself.
-          rewrite cats0.
-            by apply: H.
-            
-              by apply: filter_normalize_swap.
-                by apply: uniq_get_possible_types.
-                  by apply/allP; apply: in_possible_types_is_object.
-
-                  move/ohead_in: Hv => Hin.
-                  move: (@neighbours_are_subtype_of_field Vals s g u (Field name2 arguments2) f Heq0 v Hin).
-                    by rewrite Hrty.
-
-
-      * rewrite filter_normalize_swap filter_filter_absorb // H0 //; congr cons; congr pair; congr Array.
-        apply/eq_in_map => v Hin; congr Response.Object.
-        rewrite -filter_normalize_swap find_filter_nil.
-        simp merge_selection_sets => /=; rewrite cats0 exec_inlined_func.
-        exec.
-        have Hvin : v \in g.(nodes) by apply: neighbours_are_in_nodes; exact: Hin.
+    - simp merge_selection_sets => /=; rewrite cats0.
+      congr cons; congr pair; congr Response.Object.
+      rewrite exec_inlined_func //.
+      simp execute_selection_set.
+      have Hvin : v \in g.(nodes).
+      apply: ohead_in_nodes; last by apply: Hv.
+        by apply/allP; apply: neighbours_are_in_nodes.
         have Hvobj := (node_in_graph_has_object_type Hvin).
         have -> /= : does_fragment_type_apply s v.(ntype) v.(ntype) by apply: object_applies_to_itself.
         rewrite cats0.
           by apply: H.
+          
             by apply: filter_normalize_swap.
               by apply: uniq_get_possible_types.
-                by apply/allP; apply: in_possible_types_is_object.  
-
+                by apply/allP; apply: in_possible_types_is_object.
+                
+                move/ohead_in: Hv => Hin.
                 move: (@neighbours_are_subtype_of_field Vals s g u (Field name2 arguments2) f Heq0 v Hin).
                   by rewrite Hrty.
+                  
+
+    - congr cons; congr pair; congr Array.
+      apply/eq_in_map => v Hin; congr Response.Object.
+      simp merge_selection_sets => /=; rewrite cats0 exec_inlined_func.
+      simp execute_selection_set.
+      have Hvin : v \in g.(nodes) by apply: neighbours_are_in_nodes; exact: Hin.
+      have Hvobj := (node_in_graph_has_object_type Hvin).
+      have -> /= : does_fragment_type_apply s v.(ntype) v.(ntype) by apply: object_applies_to_itself.
+      rewrite cats0.
+        by apply: H.
+          by apply: filter_normalize_swap.
+            by apply: uniq_get_possible_types.
+              by apply/allP; apply: in_possible_types_is_object.  
+              
+              move: (@neighbours_are_subtype_of_field Vals s g u (Field name2 arguments2) f Heq0 v Hin).
+                by rewrite Hrty.
   Qed.
 
 
@@ -377,7 +412,7 @@ Section Theory.
           by apply: uniq_get_possible_types.
             by apply/allP; apply: in_possible_types_is_object.
             
-            exec.
+            simp execute_selection_set.
             have -> /= : does_fragment_type_apply s u.(ntype) u.(ntype)
               by apply: object_applies_to_itself; apply: (in_possible_types_is_object Hin).
             rewrite cats0.
@@ -418,7 +453,169 @@ Section Theory.
   Qed.
 
 
+  
+  Transparent is_field.
 
+  (**
+     This lemma states that [execute_selection_set2] distributes over list concatenation.
+   *)
+  Lemma exec2_cat u φ β :
+    s, g ⊢ ≪ φ ++ β ≫ in u = s, g ⊢ ≪ φ ≫ in u ++ s, g ⊢ ≪ β ≫ in u.
+  Proof.
+    move: {2}(queries_size _) (leqnn (queries_size φ)) => n.
+    elim: n φ β => /= [| n IH] φ β; first by rewrite leqn0 => /queries_size_0_nil ->.
+    case: φ => // q φ; case_query q; simp query_size => Hleq; exec2; rewrite -/cat ?IH //; leq_queries_size.
+      by case does_fragment_type_apply => /=; rewrite ?catA; apply: IH; leq_queries_size.
+  Qed.
+
+
+  
+
+  (**
+     This lemma states that evaluating a list of inline fragments in which 
+     all have a type condition that does not apply to the node's type will result 
+     in an empty response ([execute_selection_set2]).
+   *)
+  Lemma exec_inlines_nil φ u :
+    all (fun q => q.(is_inline_fragment)) φ ->
+     all (fun q => if q is on t { _ } then
+                 ~~ does_fragment_type_apply s u.(ntype) t
+               else
+                 true) φ ->
+    s, g ⊢ ⟦ φ ⟧ˢ in u = [::].
+  Proof.
+    funelim (s, g ⊢ ⟦ φ ⟧ˢ in u) => //=; bcase.
+      by rewrite Heq in Hb0.
+    by apply: H => //; intros; apply: (Hnappl q) => //; apply: mem_tail.
+  Qed.
+
+ 
+  (**
+     This lemma states that evaluating a list of inline fragments in which 
+     all have a type condition that does not apply to the node's type will result 
+     in an empty response ([execute_selection_set2]).
+   *)
+  Lemma exec2_inlines_nil φ u :
+    all (fun q => q.(is_inline_fragment)) φ ->
+    all (fun q => if q is on t { _ } then
+                 ~~ does_fragment_type_apply s u.(ntype) t
+               else
+                 true) φ ->
+    s, g ⊢ ≪ φ ≫ in u = [::].
+  Proof.
+    funelim (s, g ⊢ ≪ φ ≫ in u) => //=; bcase.
+      by rewrite Heq in Hb0.
+    by apply: H => //; intros; apply: (Hnappl q) => //; apply: mem_tail.
+  Qed.
+  
+ 
+
+  (**
+     This lemma states that evaluating a concatenation of two lists [φ] and [β], 
+     where [β] consists of inline fragments whose type condition does not apply 
+     to the node's type, is equal to just evaluatin [φ] by itself ([β] does 
+     not produce any response).
+
+     I believe this could be extended to any type of list [β], if we include 
+     the notion of query conformance.
+
+     See also:
+     - [exec_equivalence]
+   *)
+  Lemma exec_grounded_inlines_nil φ β u :
+    all (fun q => q.(is_inline_fragment)) β ->
+    all (fun q => if q is on t { _ } then
+                 ~~ does_fragment_type_apply s u.(ntype) t
+               else
+                 true) β ->
+    s, g ⊢ ⟦ φ ++ β ⟧ˢ in u = s, g ⊢  ⟦ φ ⟧ˢ in u.
+  Proof.
+    move: {2}(queries_size _) (leqnn (queries_size φ)) => n.
+    elim: n φ β u => /= [| n IH] φ β u; first by rewrite leqn0 => /queries_size_0_nil -> /=; apply: exec_inlines_nil.
+    case: φ => //= [_ | q φ]; first by apply: exec_inlines_nil.
+    case_query q; simp query_size => Hleq; intros; exec; rewrite ?filter_queries_with_label_cat ?find_queries_with_label_cat ?[find_queries_with_label _ _ _ β]find_fragment_not_applies_is_nil // ?cats0 //.
+    all: do ? congr cons.
+    all: do ? [apply: IH => //; leq_queries_size].
+    all: do ? by apply: filter_preserves_inlines.
+    all: do ? by apply: filter_preserves_fragment_not_applies.
+
+    - by rewrite catA; apply: IH; leq_queries_size.
+  Qed.   
+
+
+  (**
+     This lemma states that if there is no grounded fragment with type condition 
+     [ty], then no fragment applies to [ty].
+
+     The idea is that grounded fragments have Object types as type condition and 
+     the only way for an Object type to apply to another is that they are the same.
+     
+     See also:
+     - [exec_equivalence]
+   *)
+  Lemma find_frags_nil_then_N_applies φ ty :
+    find_fragment_with_type_condition ty φ = [::] ->
+    are_grounded_inlines s φ ->
+    all (fun q => if q is on t { _ } then
+                 ~~ does_fragment_type_apply s ty t
+               else
+                 true) φ.
+  Proof.
+    elim: φ => // q φ IH; case_query q => //.
+    simp find_fragment_with_type_condition; case: eqP => //= /eqP Hneq Hfind.
+    simp is_grounded; bcase.
+    move: Hb2; bcase.
+    rewrite /does_fragment_type_apply Hb0 Hneq.
+    apply_andP; by apply: IH.
+  Qed.
+    
+      
+  (**
+     This theorem states that in the presence of a query in normal form, 
+     both the semantics with collection and the simplified semantics are 
+     equivalent.
+
+     ---- 
+     See also :
+     - [execute_selection_set]
+     - [execute_selection_set2]
+     
+   *)
+  Theorem exec_equivalence u φ :
+    are_grounded s φ ->
+    are_non_redundant φ -> 
+    s, g ⊢ ⟦ φ ⟧ˢ in u = s, g ⊢ ≪ φ ≫ in u.
+  Proof.
+    move: {2}(queries_size _) (leqnn (queries_size φ)) => n.
+    elim: n φ u => /= [| n IH] φ u; first by rewrite leqn0 => /queries_size_0_nil ->.
+    case: φ => // q φ; case_query q; simp query_size => Hleq; grounding; non_red => /=; bcase; exec; exec2.
+
+    all: do ?[by apply: IH => //=; grounding].
+    
+    all: do ? [rewrite filter_find_fields_nil_is_nil in IH *; [
+               | by move: Hb2; rewrite are_grounded_fields_E; bcase
+               | by apply/eqP ] ].
+    all: do ? congr cons.
+    all: do ? [by apply: IH; leq_queries_size; [grounding | non_red] ].     
+
+    all: do ? [congr pair; congr Array; apply/eq_in_map=> v Hin; congr Response.Object].
+    all: do ? [rewrite find_queries_nil_if_find_fields_nil// /merge_selection_sets /= ?cats0 in IH *; last by apply/eqP].
+    all: do ? by rewrite IH //; leq_queries_size.
+      
+    - move: Hb1; simp is_grounded; bcase.
+      have Htyeq : u.(ntype) = t.
+        by apply/eqP; move: Hfapplies; rewrite /does_fragment_type_apply Hb1.
+        rewrite exec_grounded_inlines_nil ?exec2_cat.
+        have -> /= := (exec2_inlines_nil φ).
+          by rewrite cats0; apply: IH => //; leq_queries_size; grounding.
+
+          all: do ? by move: Hb2; rewrite are_grounded_inlines_E; case/andP.
+
+          all: do ? by rewrite -Htyeq in Hb1 Hb0; apply: find_frags_nil_then_N_applies => //=; apply/eqP.                
+  Qed.
+
+
+  
 
 End Theory.
 
